read' must eval to a valid location

theories/CachedWaitFree.v
@@ -31,14 +31,18 @@ Definition new_big_atomic (n : nat) : val :=
 
 Definition read' (n : nat) : val :=
   λ: "l",
+    let: "l'" := NewProph in
     let: "ver" := !"l" in
     let: "data" := array_clone ("l" +ₗ #2) #n in
-    let: "p" := NewProph in
     let: "backup" := !("l" +ₗ #1) in
-    if: (Fst "backup") && Resolve (!"l" = "ver") "p" #() then
+    if: (Fst "backup") && (!"l" = "ver") then (
+      resolve_proph: "l'" to: "data";;
       ("data", "backup", "ver")
-    else
-      (array_clone (Snd "backup") #n, "backup", "ver").
+    ) else (
+      let: "copy" := array_clone (Snd "backup") #n in
+      resolve_proph: "l'" to: "copy";;
+      ("copy", "backup", "ver")
+    ).
 
 Definition read (n : nat) : val := λ: "l", Fst (Fst (read' n "l")).
 
@@ -1035,9 +1039,15 @@ Lemma index_auth_frag_agree (γ : gname) (i : nat) (l : loc) (index : list loc) 
       iApply "HΦ". by iFrame.
   Qed.
 
-  Definition extract_result (vs : list (val * val)) : option bool :=
+  Definition extract_bool (vs : list (val * val)) : option bool :=
     match vs with
     | (LitV (LitBool b), _) :: _ => Some b
+    | _ => None
+    end.
+
+  Definition extract_loc (vs : list (val * val)) : option loc :=
+    match vs with
+    | (_, LitV (LitLoc l)) :: _ => Some l
     | _ => None
     end.
 
@@ -1063,9 +1073,15 @@ Lemma index_auth_frag_agree (γ : gname) (i : nat) (l : loc) (index : list loc) 
   Proof.
     iIntros (Hpos) "#Hinv %Φ AU".
     wp_rec.
+    wp_apply wp_new_proph.
+    { done. }
+    iIntros (pvs p) "Hproph".
+    wp_pures.
     wp_bind (! _)%E.
     iInv cached_wfN as "(%ver & %log & %actual & %cache & %valid & %backup & %backup' & %requests & %index & >Hver & >Hbackup & >Hγ & >#□Hbackup & >%Hindex & >%Hvalidated & >Hregistry & Hreginv & >%Hlenactual & >%Hlencache & Hlog & >%Hlogged & >●Hlog & >%Hlenᵢ & >%Hnodup & >%Hrange & Hlock)" "Hcl".
     wp_load.
+    (* Consider whether initial version is even *)
+    (* If the version is odd, the speculative read will always fail *)
     destruct (Nat.even ver) eqn:Heven.
     - iDestruct "Hlock" as "(Hγᵢ & Hγᵥ & %Hunlocked & Hcache)".
       iPoseProof (mono_nat_lb_own_get with "Hγᵥ") as "#Hlb".
@@ -1076,7 +1092,7 @@ Lemma index_auth_frag_agree (γ : gname) (i : nat) (l : loc) (index : list loc) 
       { eauto. }
       iMod (index_frag_alloc with "Hγᵢ") as "[●Hindex #◯Hindex]".
       { by rewrite last_lookup Hlenᵢ /= in Hindex. }
-      iMod ("Hcl" with "[-AU]") as "_".
+      iMod ("Hcl" with "[-AU Hproph]") as "_".
       { rewrite /cached_wf_inv.
         iExists ver, log, actual, cache, valid, backup, backup', requests, index.
         rewrite Heven. iFrame "∗ # %". }
@@ -1086,20 +1102,227 @@ Lemma index_auth_frag_agree (γ : gname) (i : nat) (l : loc) (index : list loc) 
       { done. }
       iIntros (vers vdst dst) "(Hdst & %Hlen' & %Hsorted & %Hbound & Hcons)".
       wp_pures.
-      wp_apply wp_new_proph.
-      { done. }
-      iIntros (pvs p) "Hproph".
-      wp_pures.
       wp_bind (! _)%E.
       iInv cached_wfN as "(%ver' & %log' & %actual' & %cache' & %valid' & %backup₁ & %backup₁' & %requests' & %index' & >Hver & >Hbackup & >Hγ & >#□Hbackup₁ & >%Hindex' & >%Hvalidated' & >Hregistry & Hreginv & >%Hlenactual' & >%Hlencache' & Hlog & >%Hlogged' & >●Hlog & >%Hlenᵢ' & >%Hnodup' & >%Hrange' & Hlock)" "Hcl".
       wp_load.
+      destruct (extract_loc pvs) as [|] eqn:Hres; first last.
+      { iMod ("Hcl" with "[-Hdst Hproph]") as "_".
+        { iExists ver', log', actual', cache', valid', backup₁, backup₁', requests', index'.
+          iFrame "∗ # %". }
+        iModIntro.
+        wp_pures.
+        destruct valid'.
+        { wp_pures.
+          wp_bind (! _)%E.
+          iInv cached_wfN as "(%ver'' & %log'' & %actual'' & %cache'' & %valid'' & %backup₂ & %backup₂' & %requests'' & %index'' & >Hver & >Hbackup & >Hγ & >#□Hbackup₂ & >%Hindex'' & >%Hvalidated'' & >Hregistry & Hreginv & >%Hlenactual'' & >%Hlencache'' & Hlog & >%Hlogged'' & >●Hlog & >%Hlenᵢ'' & >%Hnodup'' & >%Hrange'' & Hlock)" "Hcl".
+          wp_load.
+        iMod ("Hcl" with "[-Hdst Hproph]") as "_".
+        { iExists ver'', log'', actual'', cache'', valid'', backup₂, backup₂', requests'', index''.
+          iFrame "∗ # %". }
+        iModIntro.
+        wp_pures.
+        destruct (decide (ver'' = ver)) as [<- | Hne].
+        - rewrite bool_decide_eq_true_2; last done.
+          wp_pures.
+          wp_bind (Resolve _ _ _).
+          wp_apply (wp_resolve with "Hproph").
+          { done. }
+          wp_pures.
+          iModIntro.
+          iIntros (pvs' ->) "Hproph //".
+        - rewrite bool_decide_eq_false_2; first last.
+          { intros [=]. simplify_eq. }
+          wp_pures.
+          wp_apply (wp_array_clone_persistent with "□Hbackup₁").
+          { lia. }
+          { lia. }
+          iIntros (l') "_".
+          wp_pures.
+          wp_bind (Resolve _ _ _).
+          wp_apply (wp_resolve with "Hproph").
+          { done. }
+          wp_pures.
+          iModIntro.
+          iIntros (pvs' ->) "Hproph //". }
+        case_bool_decide
+
+          
+        }
+      
       iMod "AU" as (vs') "[Hγ' [_ Hconsume]]".
       iCombine "Hγ Hγ'" gives %[_ <-].
-      destruct (extract_result pvs) as [[|]|] eqn:Hres.
-      + destruct valid'.
+      destruct valid'.
+      + destruct (extract_loc pvs) as [|] eqn:Hres.
         { iMod ("Hconsume" $! true dst backup₁ ver γₜ with "Hγ'") as "HΦ".
           destruct (decide (ver = ver')) as [<- | Hne]. 
           - rewrite Heven.
+            iDestruct "Hlock" as "(Hγᵢ & Hγᵥ & %Hunlocked' & Hcache)".
+            rewrite /log_frag_own.
+            iPoseProof (log_auth_frag_agree with "●Hlog ◯Hlog") as "%Hlookup".
+            destruct Hvalidated' as (_ & <- & <-).
+            rewrite last_lookup Hlenᵢ' /= in Hindex'.
+            iAssert (⌜cache = vdst⌝)%I with "[Hcons Hγᵥ]" as "<-".
+            { iApply pure_mono.
+              { by apply list_eq_same_length. }
+              rewrite big_sepL2_forall.
+              iDestruct "Hcons" as "[%Heq #Hcons]".
+              iIntros (i v v' Hlt Hv Hv').
+              assert (i < length vers) as [ver' Hver']%lookup_lt_is_Some by lia.
+              iPoseProof ("Hcons" with "[//] [//]") as "[#Hlb' #Hfrag]".
+              assert (ver ≤ ver') as Hle by (by eapply Forall_lookup).
+              iPoseProof (mono_nat_lb_own_valid with "Hγᵥ Hlb'") as "[%Hq %Hge]".
+              assert (ver = ver') as <- by lia.
+              clear Hle Hge.
+              iPoseProof ("Hfrag" with "[]") as "(%l' & %γₜ' & %vs' & #◯Hindex' & #◯Hlog' & %Hlookup')".
+              { by rewrite -Nat.even_spec. }
+              iCombine "◯Hindex ◯Hindex'" gives %Hvalid%auth_frag_op_valid_1.
+              rewrite singleton_op singleton_valid in Hvalid.
+              apply to_agree_op_inv_L in Hvalid as <-.
+              iCombine "◯Hlog ◯Hlog'" gives %Hvalid%auth_frag_op_valid_1.
+              rewrite singleton_op singleton_valid in Hvalid.
+              apply to_agree_op_inv_L in Hvalid as [=<-<-].
+              simplify_eq. iPureIntro. apply (inj Some). by rewrite -Hv -Hlookup'. }
+            rewrite last_lookup Hlenᵢ /= in Hindex.
+            iDestruct (index_auth_frag_agree with "Hγᵢ ◯Hindex") as "%H".
+            simplify_eq.
+            iMod ("Hcl" with "[-HΦ Hdst Hproph]") as "_".
+            { iExists ver, log', actual', actual', true, backup₁, backup₁, requests', index'.
+              iFrame "∗ # %". rewrite last_lookup Hlenᵢ' Heven /=. iFrame "∗ # %".
+              iIntros "!> !%". split; last done. by rewrite -Nat.even_spec. }
+            iModIntro.
+            wp_pures.
+            wp_bind (! _)%E.
+            iInv cached_wfN as "(%ver' & %log'' & %actual'' & %cache' & %valid' & %backup₂ & %backup₂' & %requests'' & %index'' & >Hver & >Hbackup & >Hγ & >#□Hbackup₂ & >%Hindex'' & >%Hvalidated'' & >Hregistry & Hreginv & >%Hlenactual'' & >%Hlencache'' & Hlog & >%Hlogged'' & >●Hlog & >%Hlenᵢ'' & >%Hnodup'' & >%Hrange'' & Hlock)" "Hcl".
+            wp_load.
+            iMod ("Hcl" with "[-HΦ Hdst Hproph]") as "_".
+            { iExists ver', log'', actual'', cache', valid', backup₂, backup₂', requests'', index''.
+              iFrame "∗ # %". }
+            iModIntro.
+            wp_pures.
+            wp_apply (wp_resolve with "Hproph").
+            { done. }
+            wp_pures.
+            iModIntro.
+            iIntros (pvs' ->) "Hpvs".
+            simpl in *. simplify_eq.
+            rewrite bool_decide_eq_true in Hres.
+            simplify_eq.
+            rewrite bool_decide_eq_true_2; last done.
+            wp_pures. iModIntro. iApply "HΦ". simpl in *. iFrame "∗ #".
+            rewrite -lookup_fmap lookup_fmap_Some in Hlogged'.
+            destruct Hlogged' as ([γ' vs'] & ? & ?). simpl in *. simplify_eq.
+            assert ((γ', actual') = (γₜ, vs)) as [=->->].
+            { apply (inj Some). by etransitivity. }
+            by iFrame "∗ %".
+          - iAssert (⌜ver < ver'⌝ ∗ mono_nat_lb_own γᵥ ver')%I as "[%Hless #Hlb']".
+            { destruct (Nat.even ver') eqn:Heven';
+              iDestruct "Hlock" as "(_ & Hγᵥ & _)";
+              iDestruct (mono_nat_lb_own_valid with "Hγᵥ Hlb") as %[_ Hle]; iSplit.
+              1, 3: (iPureIntro; lia).
+              all: iApply (mono_nat_lb_own_get with "Hγᵥ"). }
+            iMod ("Hcl" with "[-HΦ Hdst Hproph]") as "_".
+            { iExists ver', log', actual', cache', true, backup₁, backup₁', requests', index'.
+              iFrame "∗ # %". }
+            iModIntro.
+            wp_pures.
+            wp_bind (! _)%E.
+            iInv cached_wfN as "(%ver'' & %log'' & %actual'' & %cache'' & %valid' & %backup₂ & %backup₂' & %requests'' & %index'' & >Hver & >Hbackup & >Hγ & >#□Hbackup₂ & >%Hindex'' & >%Hvalidated'' & >Hregistry & Hreginv & >%Hlenactual'' & >%Hlencache'' & Hlog & >%Hlogged'' & >●Hlog & >%Hlenᵢ'' & >%Hnodup'' & >%Hrange'' & Hlock)" "Hcl".
+            wp_load.
+            iAssert (⌜ver < ver''⌝)%I as %Hless'.
+            { destruct (Nat.even ver'');
+              iDestruct "Hlock" as "(_ & Hγᵥ & _)";
+              iDestruct (mono_nat_lb_own_valid with "Hγᵥ Hlb'") as %[_ Hle'];
+              iPureIntro; lia. }
+            iMod ("Hcl" with "[-HΦ Hdst Hproph]") as "_".
+            { iExists ver'', log'', actual'', cache'', valid', backup₂, backup₂', requests'', index''.
+              iFrame "∗ # %". }
+            iModIntro.
+            wp_pures.
+            wp_apply (wp_resolve with "Hproph").
+            { done. }
+            wp_pures.
+            iModIntro.
+            iIntros (pvs' ->) "Hproph".
+            simpl in *.
+            simplify_eq.
+            rewrite bool_decide_eq_true in Hres.
+            simplify_eq. lia. }
+        { (* Version check is prophecied to fail *)
+          iMod ("Hconsume" $! true with "Hγ'") as "HΦ".
+          rewrite /log_frag_own.
+          iPoseProof (log_auth_frag_agree with "●Hlog ◯Hlog") as "%Hlookup".
+          destruct Hvalidated' as (_ & <- & <-).
+          rewrite last_lookup Hlenᵢ' /= in Hindex'.
+          rewrite last_lookup Hlenᵢ /= in Hindex.
+          destruct (Nat.even ver') eqn:Heven'.
+          - iDestruct "Hlock" as "(Hγᵢ & Hγᵥ & %Hunlocked' & Hcache)".
+            iDestruct (index_auth_frag_agree with "Hγᵢ ◯Hindex") as "%H".
+            simplify_eq.
+            iMod ("Hcl" with "[-HΦ Hdst Hproph]") as "_".
+            { iExists ver', log', actual', actual', true, backup₁, backup₁, requests', index'.
+              iFrame "∗ # %". rewrite last_lookup Hlenᵢ' Heven' /=. iFrame "∗ # %".
+              iIntros "!> !%". split; last done. by rewrite -Nat.even_spec. }
+            iModIntro.
+            wp_pures.
+            wp_bind (! _)%E.
+            iInv cached_wfN as "(%ver'' & %log'' & %actual'' & %cache' & %valid' & %backup₂ & %backup₂' & %requests'' & %index'' & >Hver & >Hbackup & >Hγ & >#□Hbackup₂ & >%Hindex'' & >%Hvalidated'' & >Hregistry & Hreginv & >%Hlenactual'' & >%Hlencache'' & Hlog & >%Hlogged'' & >●Hlog & >%Hlenᵢ'' & >%Hnodup'' & >%Hrange'' & Hlock)" "Hcl".
+              wp_load.
+            iMod ("Hcl" with "[-HΦ Hdst Hproph]") as "_".
+            { iExists ver'', log'', actual'', cache', valid', backup₂, backup₂', requests'', index''.
+              iFrame "∗ # %". }
+            iModIntro.
+            wp_pures.
+            wp_apply (wp_resolve with "Hproph").
+            { done. }
+            wp_pures.
+            iModIntro.
+            iIntros (pvs' ->) "Hproph".
+            simpl in *.
+            simplify_eq.
+            rewrite bool_decide_eq_false_2; first last.
+            { by rewrite bool_decide_eq_false in Hres. }
+            wp_pures.
+            wp_apply (wp_array_clone_persistent with "□Hbackup₁").
+            { lia. }
+            { lia. }
+            iIntros (l') "Hl'".
+            wp_pures.
+            iModIntro.
+            iApply "HΦ".
+
+          destruct (decide (ver' = ver)) as [<- | Hne].
+          { wp_pures.
+            wp_apply (wp_resolve with "Hproph").
+            { done. }
+            wp_pures.
+            iModIntro.
+            iIntros (pvs' ->) "Hproph".
+            simpl in *. simplify_eq. rewrite bool_decide_eq_false in Hres.
+            rewrite bool_decide_eq_false_2; first last.
+            { done. }
+            assert (ver'' ≠ ver') as Hne.
+            { congruence. }
+            wp_pures.
+
+            rewrite bool_decide_eq_true_2; last done.
+            iIntros (pvs' ->) "Hproph".
+            wp_pures. iModIntro. iApply "HΦ". simpl in *. iFrame "∗ #".
+            rewrite -lookup_fmap lookup_fmap_Some in Hlogged'.
+            destruct Hlogged' as ([γ' vs'] & ? & ?). simpl in *. simplify_eq.
+            assert ((γ', actual') = (γₜ, vs)) as [=->->].
+            { apply (inj Some). by etransitivity. }
+            by iFrame "∗ %". }
+          { wp_pures.
+            wp_apply (wp_resolve with "Hproph").
+            { done. }
+            wp_pures.
+            iModIntro.
+            iIntros (pvs' ->) "Hproph".
+            simpl in *.
+            simplify_eq.
+            rewrite bool_decide_eq_true in Hres.
+            simplify_eq. }
+          rewrite Heven.
             iDestruct "Hlock" as "(Hγᵢ & Hγᵥ & %Hunlocked' & Hcache)".
             rewrite /log_frag_own.
             iPoseProof (log_auth_frag_agree with "●Hlog ◯Hlog") as "%Hlookup".
@@ -1184,22 +1407,23 @@ Lemma index_auth_frag_agree (γ : gname) (i : nat) (l : loc) (index : list loc) 
             iAssert (⌜ver < ver''⌝)%I as %Hless'.
             { destruct (Nat.even ver'');
               iDestruct "Hlock" as "(_ & Hγᵥ & _)";
-              iDestruct (mono_nat_lb_own_valid with "Hγᵥ Hlb") as %[_ Hle'];
+              iDestruct (mono_nat_lb_own_valid with "Hγᵥ Hlb'") as %[_ Hle'];
               iPureIntro; lia. }
             iMod ("Hcl" with "[-HΦ Hdst Hproph]") as "_".
             { iExists ver'', log'', actual'', cache'', valid', backup₂, backup₂', requests'', index''.
               iFrame "∗ # %". }
-              iModIntro.
-              wp_pures.
-              wp_apply (wp_resolve with "Hproph").
-              { done. }
-              wp_pures.
-              iModIntro.
-              iIntros (pvs' ->) "Hproph".
-              simpl in *.
-              simplify_eq.
-              rewrite bool_decide_eq_true in Hres.
-              simplify_eq. lia.
+            iModIntro.
+            wp_pures.
+            wp_apply (wp_resolve with "Hproph").
+            { done. }
+            wp_pures.
+            iModIntro.
+            iIntros (pvs' ->) "Hproph".
+            simpl in *.
+            simplify_eq.
+            rewrite bool_decide_eq_true in Hres.
+            simplify_eq. lia. }
+      + 
 
               rewrite bool_decide_eq_false_2; first last.
               { intros [=]. lia. }
